working on adequacy

theories/program_logic/adequacy.v
@@ -1,3 +1,643 @@
+From iris.proofmode Require Import tactics.
+From iris.algebra Require Import gmap auth agree gset coPset.
+From iris.base_logic.lib Require Import wsat.
+From aneris.prelude Require Import quantifiers iris_extraction.
+From aneris.program_logic Require Export weakestpre.
+
+Set Default Proof Using "Type".
+Import uPred.
+
+Record execution_trace Λ := {
+  extr_path : list (cfg Λ);
+  extr_obs : list (list (observation Λ)); }.
+
+Arguments extr_path {_} _.
+Arguments extr_obs {_} _.
+
+Record auxiliary_trace (AS : Type) := {
+  auxtr_path : list AS; }.
+
+Arguments auxtr_path {_} _.
+
+Section execution_trace.
+  Context {Λ : language}.
+
+  Definition singleton_exec (c : cfg Λ) : execution_trace Λ :=
+    {| extr_path := [c]; extr_obs := []; |}.
+
+  Definition exec_starts_in (e : execution_trace Λ) (c : cfg Λ) : Prop :=
+    hd_error (extr_path e) = Some c.
+
+  Definition exec_ends_in (e : execution_trace Λ) (c : cfg Λ) : Prop :=
+    last (extr_path e) = Some c.
+
+  Lemma singleton_exec_starts_in c : exec_starts_in (singleton_exec c) c.
+  Proof. done. Qed.
+
+  Lemma singleton_exec_ends_in c : exec_ends_in (singleton_exec c) c.
+  Proof. done. Qed.
+
+  Lemma exec_ends_in_inj e c c' :
+    exec_ends_in e c → exec_ends_in e c' → c = c'.
+  Proof. rewrite /exec_ends_in; intros ->; congruence. Qed.
+
+  Fixpoint valid_extr_path
+           (ep : list (cfg Λ)) (obs : list (list (observation Λ))) : Prop :=
+    match ep with
+    | [] => obs = []
+    | c :: ep' =>
+      match ep' with
+      | [] => obs = []
+      | c' :: ep'' =>
+        ∃ κ obs', obs = κ :: obs' ∧ step c κ c' ∧ valid_extr_path ep' obs'
+      end
+    end.
+
+  Definition valid_exec (e : execution_trace Λ) : Prop :=
+    valid_extr_path (extr_path e) (extr_obs e).
+
+  Lemma valid_singleton_exec c : valid_exec (singleton_exec c).
+  Proof. done. Qed.
+
+  Definition exec_extend (e : execution_trace Λ) (c : cfg Λ)
+             (κ : list (observation Λ)) :=
+    {| extr_path := extr_path e ++ [c];
+       extr_obs := extr_obs e ++ [κ]; |}.
+
+  Lemma exec_extend_starts_in e c' c κ :
+    exec_starts_in e c' → exec_starts_in (exec_extend e c κ) c'.
+  Proof.
+    rewrite /exec_starts_in /exec_extend /=; intros Hec'.
+    assert (extr_path e = c' :: tail (extr_path e)) as ->
+        by by apply hd_error_tl_repr.
+    done.
+  Qed.
+
+  Lemma exec_extend_ends_in e c κ : exec_ends_in (exec_extend e c κ) c.
+  Proof. apply last_snoc. Qed.
+
+  Definition exec_get_obs (e : execution_trace Λ) :=
+    fold_right (λ κ κs, κ ++ κs) [] (extr_obs e).
+
+  Lemma exec_extend_get_obs e c κ :
+    exec_get_obs (exec_extend e c κ) = exec_get_obs e ++ κ.
+  Proof.
+    rewrite /exec_get_obs /=.
+    revert κ.
+    induction (extr_obs e) as [|κ' obs IHobs]; intros κ; simpl.
+    { rewrite app_nil_r //. }
+    rewrite IHobs -!assoc_L //=.
+  Qed.
+
+  Lemma extend_valid_exec e c κ c':
+    valid_exec e →
+    exec_ends_in e c →
+    step c κ c' →
+    valid_exec (exec_extend e c' κ).
+  Proof.
+    destruct e as [ep eo]; rewrite /valid_exec /exec_ends_in /=.
+    revert eo.
+    induction ep as [|d ep IHep];
+      intros eo Hvl Hend Hstp; first done.
+    assert (ep = nil → d = c) as Hep1 by by intros ->; simplify_eq/=.
+    assert (ep ≠ nil → last ep = Some c) as Hep2 by by destruct ep.
+    destruct ep; simpl.
+    { simplify_eq/=; eexists κ, _; done. }
+    destruct Hvl as (κ' & eo' & -> & Hdstp & Hvl).
+    eexists κ', _; split_and!; [done|done|].
+    eapply IHep; eauto.
+  Qed.
+
+End execution_trace.
+
+Section auxiliary_trace.
+  Context {AS : Type}.
+
+  Definition singleton_sim (st : AS) : auxiliary_trace AS :=
+    {| auxtr_path := [st]; |}.
+
+  Definition sim_starts_in (sm : auxiliary_trace AS) (st : AS) : Prop :=
+    hd_error (auxtr_path sm) = Some st.
+
+  Definition sim_ends_in (sm : auxiliary_trace AS) (st : AS) : Prop :=
+    last (auxtr_path sm) = Some st.
+
+  Lemma singleton_sim_starts_in st : sim_starts_in (singleton_sim st) st.
+  Proof. done. Qed.
+
+  Lemma singleton_sim_ends_in st : sim_ends_in (singleton_sim st) st.
+  Proof. done. Qed.
+
+  Lemma sim_ends_in_inj sm st st' :
+    sim_ends_in sm st → sim_ends_in sm st' → st = st'.
+  Proof. rewrite /sim_ends_in; intros ->; congruence. Qed.
+
+  Fixpoint valid_auxtr_path (sm : list AS) : Prop :=
+    match sm with
+    | [] => True
+    | st :: sm' =>
+      match sm' with
+      | [] => True
+      | st' :: sm'' => M st st' ∧ valid_auxtr_path sm'
+      end
+    end.
+
+  Definition valid_sim (sm : auxiliary_trace M) : Prop :=
+    valid_auxtr_path (auxtr_path sm).
+
+  Lemma valid_singleton_sim st : valid_sim (singleton_sim st).
+  Proof. done. Qed.
+
+  Definition sim_extend (sm : auxiliary_trace M) (st : M) :=
+    {| auxtr_path := auxtr_path sm ++ [st]; |}.
+
+  Lemma sim_extend_starts_in sm st' st :
+    sim_starts_in sm st' → sim_starts_in (sim_extend sm st) st'.
+  Proof.
+    rewrite /sim_starts_in /sim_extend /=; intros Hec'.
+    assert (auxtr_path sm = st' :: tail (auxtr_path sm)) as ->
+        by by apply hd_error_tl_repr.
+    done.
+  Qed.
+
+  Lemma sim_extend_ends_in sm st : sim_ends_in (sim_extend sm st) st.
+  Proof. apply last_snoc. Qed.
+
+  Lemma sim_valid_exec sm st st':
+    valid_sim sm →
+    sim_ends_in sm st →
+    M st st' →
+    valid_sim (sim_extend sm st').
+  Proof.
+    destruct sm as [smp]; rewrite /valid_sim /sim_ends_in /=.
+    induction smp as [|st'' smp IHsmp];
+      intros Hvl Hend Hstp; first done.
+    assert (smp = nil → st'' = st) as Hep1 by by intros ->; simplify_eq/=.
+    assert (smp ≠ nil → last smp = Some st) as Hep2 by by destruct smp.
+    destruct smp; simpl.
+    { simplify_eq/=; done. }
+    destruct Hvl as [? ?]; split; first done.
+    eapply IHsmp; eauto.
+  Qed.
+
+End auxiliary_trace.
+
+Definition wptp_pre Σ M {Λ} (s : stuckness)
+           (φ : execution_trace Λ → auxiliary_trace M → Prop)
+           (wptp : execution_trace Λ -d> auxiliary_trace M -d> iPropO Σ) :
+  execution_trace Λ -d> auxiliary_trace M -d> iPropO Σ :=
+  (λ ex sm,
+  ⌜valid_exec ex⌝ →
+  ⌜φ ex sm⌝ →
+  ∀ c c' κ st,
+    ⌜exec_ends_in ex c⌝ →
+    ⌜sim_ends_in sm st⌝ →
+    ⌜step c κ c'⌝ →
+    ▷ ▷ (∃ st', ⌜st' = st ∨ M st st'⌝ ∧
+                ⌜φ (exec_extend ex c' κ) (sim_extend sm st')⌝ ∧
+                wptp (exec_extend ex c' κ) (sim_extend sm st')))%I.
+
+Local Instance wp_pre_contractive Σ M Λ s φ :
+  Contractive (@wptp_pre Σ M Λ s φ).
+Proof.
+  rewrite /wptp_pre=> n wp wp' Hwp ex sm.
+  repeat (f_contractive || f_equiv); apply dist_S; apply Hwp.
+Qed.
+
+Definition wptp Σ M {Λ} (s : stuckness) (φ : execution_trace Λ → auxiliary_trace M → Prop) :
+  execution_trace Λ → auxiliary_trace M → iProp Σ := fixpoint (wptp_pre Σ M s φ).
+
+Instance is_except_0_wptp {Σ} M Λ s φ exp sm:
+  IsExcept0 (@wptp Σ Λ M s φ exp sm).
+Proof.
+  rewrite /IsExcept0; iIntros "H".
+  rewrite /wptp (fixpoint_unfold (wptp_pre _ _ _ _) _ _).
+  iIntros (? ? ? ? ? ? ? ? ?).
+  iMod "H".
+  iApply "H"; done.
+Qed.
+
+Global Instance wptp_plain Σ M {Λ} s φ ex sm : Plain (@wptp Σ M Λ s φ ex sm).
+Proof.
+  rewrite /Plain.
+  iIntros "H".
+  iLöb as "IH" forall (ex sm).
+  rewrite /wptp (fixpoint_unfold (wptp_pre _ _ _ _) _ _).
+  rewrite {3 5}/wptp_pre.
+  iIntros (? ? c ? ? ? ? ? ?).
+  iDestruct ("H" with "[] [] [] [] []") as "H"; [done|done|done|done|done|].
+  do 2 (iApply later_plainly_1; iNext).
+  iDestruct "H" as (st') "(#Hst' & #Hφ & H)".
+  iExists _.
+  iSplitR; first by iClear "IH"; iModIntro.
+  iSplitR; first by iClear "IH"; iModIntro.
+  iApply "IH"; done.
+Qed.
+
+Lemma wp_take_step `{!irisG Λ Σ M} s n st Φ e1 σ1 κ e2 σ2 efs κs :
+  prim_step e1 σ1 κ e2 σ2 efs →
+  state_interp σ1 κs n st -∗
+  WP e1 @ s; ⊤ {{ v, Φ v } } ={⊤}[∅]▷=∗
+  ∃ st', ⌜st' = st ∨ M st st'⌝ ∗
+  state_interp σ2 (κs ++ κ) (length efs + n) st' ∗
+  WP e2 @ s; ⊤ {{ v, Φ v } } ∗
+  ([∗ list] ef ∈ efs, WP ef @ s; ⊤ {{ v, fork_post v }}).
+Proof.
+  iIntros (Hstp) "HSI Hwp".
+  rewrite wp_unfold /wp_pre.
+  destruct (to_val e1) eqn:He1.
+  { erewrite val_stuck in He1; done. }
+  iMod ("Hwp" with "HSI") as "[Hs Hwp]".
+  iMod ("Hwp" with "[]") as "Hwp"; first done.
+  iModIntro; iNext.
+  iMod "Hwp" as (st') "(% & ? & ? & ?)".
+  iModIntro; iExists _; iFrame; done.
+Qed.
+
+Lemma wp_not_stuck `{!irisG Λ Σ M} e σ κs s Φ n st :
+  state_interp σ κs n st -∗
+  WP e @ s; ⊤ {{ v, Φ v }} ={⊤}=∗
+  state_interp σ κs n st ∗
+  WP e @ s; ⊤ {{ v, Φ v }} ∗
+  ⌜s = NotStuck → not_stuck e σ⌝.
+Proof.
+  iIntros "HSI Hwp".
+  rewrite /not_stuck assoc.
+  iApply fupd_plain_keep_r; iFrame.
+  iIntros "[HSI Hwp]".
+  rewrite wp_unfold /wp_pre.
+  destruct (to_val e) eqn:He.
+  - iModIntro; iPureIntro; eauto.
+  - iApply fupd_plain_mask.
+    iMod ("Hwp" $! _ [] with "HSI") as "[Hs Hwp]".
+    iModIntro; destruct s; [iDestruct "Hs" as %?|]; eauto.
+Qed.
+
+Lemma wp_other_not_stuck `{!irisG Λ Σ M} efs σ κs s Φ n st :
+  state_interp σ κs n st -∗
+  ([∗ list] e ∈ efs, WP e @ s; ⊤ {{Φ}}) ={⊤}=∗
+  state_interp σ κs n st ∗
+  ([∗ list] e ∈ efs, WP e @ s; ⊤ {{Φ}}) ∗
+  ⌜∀ e, e ∈ efs → s = NotStuck → not_stuck e σ⌝.
+Proof.
+  iIntros "HSI Hwp".
+  rewrite assoc.
+  iApply fupd_plain_keep_r; iFrame.
+  iIntros "[HSI Hwp]".
+  iIntros (e He).
+  iDestruct (big_sepL_elem_of with "Hwp") as "Hwp"; [done|].
+  iMod (wp_not_stuck with "HSI Hwp") as "(_ & _ & ?)"; done.
+Qed.
+
+Lemma wp_of_val_post `{!irisG Λ Σ M} e s Φ :
+  WP e @ s; ⊤ {{ v, Φ v }} ={⊤}=∗
+  from_option Φ True (to_val e) ∗
+  (from_option Φ True (to_val e) -∗ WP e @ s; ⊤ {{ v, Φ v }}).
+Proof.
+  iIntros "Hwp".
+  rewrite wp_unfold /wp_pre.
+  destruct (to_val e) eqn:He.
+  - iMod "Hwp"; simpl; iFrame; auto.
+  - iModIntro.
+    iSplit; first done.
+    iIntros "_"; done.
+Qed.
+
+Lemma wp_of_val_post_other `{!irisG Λ Σ M} efs s Φ :
+  ([∗ list] e ∈ efs, WP e @ s; ⊤ {{Φ}}) ={⊤}=∗
+  ([∗ list] v ∈ omap to_val efs, Φ v) ∗
+  (([∗ list] v ∈ omap to_val efs, Φ v) -∗ ([∗ list] e ∈ efs, WP e @ s; ⊤ {{Φ}})).
+Proof.
+  iIntros "Hefs".
+  iInduction efs as [|e efs IHefs] "IH"; simpl; first done.
+  iDestruct "Hefs" as "[Hwp Hefs]".
+  iMod (wp_of_val_post with "Hwp") as "[Hpost Hback]".
+  iMod ("IH" with "Hefs") as "[Hefspost Hefsback]".
+  iModIntro.
+  destruct (to_val e); simpl.
+  - iFrame.
+    iIntros "[Hpost Hefspost]".
+    iSplitL "Hpost Hback"; [iApply "Hback"|iApply "Hefsback"]; iFrame.
+  - iFrame.
+    iIntros "Hefspost".
+    iSplitL "Hback"; [iApply "Hback"|iApply "Hefsback"]; iFrame; done.
+Qed.
+
+Lemma take_step `{!irisG Λ Σ M} s Φ c κ c' κs es st :
+  step c κ c' →
+  hd_error c.1 = Some es →
+  state_interp c.2 κs (length (tail c.1)) st -∗
+  WP es @ s; ⊤ {{ v, Φ v }} -∗
+  ([∗ list] ef ∈ tail c.1, WP ef @ s; ⊤ {{ v, fork_post v }}) ={⊤}[∅]▷=∗
+  ⌜∀ e2, s = NotStuck → e2 ∈ c'.1 → not_stuck e2 c'.2⌝ ∗
+  ∃ st', ⌜st' = st ∨ M st st'⌝ ∗
+  state_interp c'.2 (κs ++ κ) (length (tail c'.1)) st' ∗
+  ∃ es', ⌜hd_error c'.1 = Some es'⌝ ∗
+    from_option Φ True (to_val es') ∗
+    ([∗ list] v ∈ omap to_val (tail c'.1), fork_post v) ∗
+    (from_option Φ True (to_val es') -∗
+      ([∗ list] v ∈ omap to_val (tail c'.1), fork_post v) -∗
+      WP es' @ s; ⊤ {{ v, Φ v }} ∗
+      ([∗ list] ef ∈ tail c'.1, WP ef @ s; ⊤ {{ v, fork_post v }})).
+Proof.
+  iIntros (Hstep Hes) "HSI Hes Hother".
+  destruct c as [[|e1 t1] σ1']; simplify_eq/=.
+  inversion Hstep as [? σ1 ? ? ? t21 t22 ? ? Hpstep]; simplify_eq/=.
+  destruct t21; simplify_eq/=.
+  - iMod (wp_take_step with "HSI Hes") as "Hwp"; [done|].
+    iModIntro; iNext; iMod "Hwp" as (st') "(% & HSI & Hwp & Hefs)".
+    iCombine "Hother" "Hefs" as "Hother".
+    rewrite -big_sepL_app.
+    iMod (wp_not_stuck with "HSI Hwp") as "(HSI & Hwp & %)".
+    iMod (wp_other_not_stuck with "HSI Hother") as "(HSI & Hother & %)".
+    iMod (wp_of_val_post with "Hwp") as "(Hpost & Hback)".
+    iMod (wp_of_val_post_other with "Hother") as "(Hpostother & Hbackother)".
+    iModIntro.
+    rewrite Nat.add_comm app_length.
+    iSplit.
+    { iIntros (? -> [->|]%elem_of_cons); auto. }
+    iExists _; iSplit; first done.
+    iFrame "HSI Hpostother".
+    iExists _; iSplit; first done.
+    iFrame.
+    iIntros "Hpost Hpostother".
+    iSplitL "Hpost Hback"; [iApply "Hback"|iApply "Hbackother"]; done.
+  - rewrite big_sepL_app /=.
+    iDestruct "Hother" as "(Ho1 & Hwp & Ho2)".
+    iMod (wp_take_step with "HSI Hwp") as "Hwp"; [done|].
+    iModIntro; iNext; iMod "Hwp" as (st') "(% & HSI & Hwp & Hefs)".
+    iAssert ([∗ list] ef ∈ (t21 ++ e2 :: t22 ++ efs),
+             WP ef @ s; ⊤ {{ v, fork_post v }})%I with "[Ho1 Hwp Ho2 Hefs]"
+      as "Hother".
+    { rewrite big_sepL_app /=; iFrame. }
+    iMod (wp_not_stuck with "HSI Hes") as "(HSI & Hes & %)".
+    iMod (wp_other_not_stuck with "HSI Hother") as "(HSI & Hother & %)".
+    iMod (wp_of_val_post with "Hes") as "(Hpostes & Hbackes)".
+    iMod (wp_of_val_post_other with "Hother") as "(Hpostother & Hbackother)".
+    iModIntro.
+    rewrite Nat.add_comm -app_length -app_assoc /= !app_length /=.
+    iSplit.
+    { iIntros (? -> [->|]%elem_of_cons); auto. }
+    iExists _; iSplit; first done.
+    iFrame "HSI Hpostother".
+    iExists _; iSplit; first done.
+    iFrame.
+    iIntros "Hpost Hpostother".
+    iSplitL "Hpost Hbackes"; [iApply "Hbackes"|iApply "Hbackother"]; done.
+Qed.
+
+Theorem wp_strong_adequacy_helper Σ M Λ `{!invPreG Σ}
+        (s: stuckness) (φ : execution_trace Λ → auxiliary_trace M → Prop) e1 σ1 κs st :
+  (∀ `{Hinv : !invG Σ},
+    ⊢ |={⊤}=> ∃
+         (stateI : state Λ → list (observation Λ) → nat → M → iProp Σ)
+         (Φ fork_post : val Λ → iProp Σ),
+       let _ : irisG Λ Σ M := IrisG _ _ _ Hinv stateI fork_post in
+       stateI σ1 κs 0 st ∗
+       WP e1 @ s; ⊤ {{ Φ }} ∗
+       □ (∀ (ex : execution_trace Λ) (sm : auxiliary_trace M) st' st'' c κ κs' t2 e2 t2' σ2,
+         ⌜exec_starts_in ex ([e1], σ1)⌝ -∗
+         ⌜sim_starts_in sm st⌝ -∗
+         ⌜exec_ends_in ex c⌝ -∗
+         ⌜sim_ends_in sm st'⌝ -∗
+         ⌜φ ex sm⌝ -∗
+         ⌜step c κ (t2, σ2)⌝ -∗
+         ⌜st'' = st' ∨ M st' st''⌝ -∗
+         ⌜t2 = e2 :: t2'⌝ -∗
+         ⌜∀ e2, s = NotStuck → e2 ∈ t2 → not_stuck e2 σ2⌝ -∗
+         stateI σ2 (κs' ++ κ) (length t2') st'' -∗
+         from_option Φ True (to_val e2) -∗
+         ([∗ list] v ∈ omap to_val t2', fork_post v) -∗
+         |={⊤, ∅}=>
+          ⌜ φ (exec_extend ex (t2, σ2) κ) (sim_extend sm st'') ⌝)) →
+  ⊢ wptp Σ M s φ (singleton_exec ([e1], σ1)) (singleton_sim st).
+Proof.
+  intros Hwp.
+  iMod wsat_alloc as (Hinv) "[Hw HE]".
+  iPoseProof Hwp as "Hwp".
+  rewrite uPred_fupd_eq /uPred_fupd_def.
+  iMod ("Hwp" with "[$Hw $HE]") as ">[Hw [HE Hwp']]".
+  iClear "Hwp".
+  iDestruct "Hwp'" as (stateI Φ fork_post) "(HSI & Hwp & #Hstep)".
+  clear Hwp.
+  set (IrisG Λ Σ M Hinv stateI fork_post).
+  pose proof (singleton_exec_starts_in ([e1], σ1)) as Hexpst.
+  pose proof (singleton_exec_ends_in ([e1], σ1)) as Hexpen.
+  pose proof (singleton_sim_starts_in st) as Hsmst.
+  pose proof (singleton_sim_ends_in st) as Hsmen.
+  set (es := e1) at 2.
+  set (est := st) at 2.
+  assert (hd_error ([e1], σ1).1 = Some es) as Hes by done.
+  change st with est in Hsmen at 2.
+  clearbody es est.
+  set (other := tail ([e1], σ1).1).
+  (* The following is annoying but if I don't include something blatantly
+     ephemeral the proofmode puts the result automatically in the persistent
+     context! *)
+  iAssert (stateI σ1 κs 0 est ∗
+           [∗ list] ef ∈ other, WP ef @ s; ⊤ {{ fork_post }})%I
+    with "[HSI]" as "[HSI Hother]"; [by iFrame|].
+  change 0 with (length other).
+  set (exp := singleton_exec ([e1], σ1)) in *.
+  set (smp := singleton_sim st) in *.
+  clearbody exp smp.
+  set ([e1], σ1) as c2 in Hexpen, Hes, other.
+  change σ1 with (c2.2) at 2.
+  clearbody c2.
+  unfold other; clear other.
+  iLöb as "IH" forall (exp smp c2 es est Hes κs Hsmen Hexpen Hexpst Hsmst)
+                      "Hwp Hother".
+  rewrite {2}/wptp (fixpoint_unfold (wptp_pre _ _ _ _) _ _).
+  iIntros (Hvl Hφ c c' κ st' Hends Hsmends Hstep).
+  pose proof (exec_ends_in_inj exp c c2 Hends Hexpen); simplify_eq.
+  pose proof (sim_ends_in_inj smp est st' Hsmen Hsmends); simplify_eq.
+  destruct c2 as [[|e2 t2] σ2]; simplify_eq/=.
+  iPoseProof (take_step _ _ ((_ :: _), _) with "[$HSI] Hwp Hother") as "Hstp";
+    [done|done|].
+  rewrite uPred_fupd_eq /uPred_fupd_def.
+  iMod ("Hstp" with "[$Hw $HE]") as ">(Hw & HE & Hstp)".
+  iNext.
+  iMod ("Hstp" with "[$Hw $HE]") as ">(Hw & HE & % & H)".
+  iDestruct "H" as (st'') "(% & HSI & H)".
+  iDestruct "H" as (es' Hes') "(Hpost & Hfpost & Hback)".
+  destruct c' as [[|e2' t2'] σ2']; simplify_eq/=.
+  iAssert (▷ ⌜φ (exec_extend exp (es' :: t2', σ2') κ) (sim_extend smp st'')⌝)%I
+    as "#Hextend".
+  { iMod ("Hstep"
+           with "[] [] [] [] [] [] [] [] [] HSI Hpost Hfpost [$Hw $HE]")
+      as ">(Hw & HE & %)"; done. }
+  iDestruct ("Hback" with "Hpost Hfpost") as "[Hes' Hother]".
+  iNext.
+  iExists _; iSplit; first done.
+  iSplit; first done.
+  iSpecialize ("IH" $! (exec_extend exp (es' :: t2', σ2') κ)
+                    (sim_extend smp st'') (es' :: t2', σ2') es' st'' with "[]");
+    [done|].
+  iApply ("IH" with "[] [] [] [] Hw HE HSI Hes' Hother");
+    eauto using exec_extend_ends_in, exec_extend_starts_in,
+    sim_extend_ends_in, sim_extend_starts_in.
+Qed.
+
+Definition monotone {A} (Ψ : (A → Prop) → (A → Prop)) :=
+  ∀ (P Q : A → Prop), (∀ x, P x → Q x) → ∀ x, Ψ P x → Ψ Q x.
+
+Definition GFX {A} (Ψ : (A → Prop) → (A → Prop)) : A → Prop :=
+  λ x, ∃ P, P x ∧ (∀ x, P x → Ψ P x).
+
+Lemma GFX_post_fixpoint {A} (Ψ : (A → Prop) → (A → Prop)) :
+  monotone Ψ → ∀ x, GFX Ψ x → Ψ (GFX Ψ) x.
+Proof.
+  intros Hmono x (P & HP & HΨP).
+  eapply Hmono; [|by apply HΨP].
+  intros; exists P; split; auto.
+Qed.
+
+Lemma GFX_fixpoint {A} (Ψ : (A → Prop) → (A → Prop)) :
+  monotone Ψ → ∀ x, Ψ (GFX Ψ) x ↔ GFX Ψ x.
+Proof.
+  intros Hmono x; split.
+  - intros HΨ.
+    exists (Ψ (GFX Ψ)); split; first done.
+    intros ? ?; eapply Hmono; last done.
+    apply GFX_post_fixpoint; done.
+  - apply GFX_post_fixpoint; done.
+Qed.
+
+Definition pure_wptp_pre {Λ M} (φ : execution_trace Λ → auxiliary_trace M → Prop)
+           (pure_wptp : execution_trace Λ → auxiliary_trace M → Prop) :
+  execution_trace Λ → auxiliary_trace M → Prop :=
+  λ ex sm,
+  valid_exec ex →
+  φ ex sm →
+  ∀ c c' κ st,
+    exec_ends_in ex c →
+    sim_ends_in sm st →
+    step c κ c' →
+    ∃ st', (st' = st ∨ M st st') ∧
+           φ (exec_extend ex c' κ) (sim_extend sm st') ∧
+           pure_wptp (exec_extend ex c' κ) (sim_extend sm st').
+
+Lemma pure_wptp_pre_mono {Λ M} (φ : execution_trace Λ → auxiliary_trace M → Prop) :
+  monotone
+    (λ ψ (exsm : execution_trace Λ * auxiliary_trace M),
+     (pure_wptp_pre φ (λ ex sm, ψ (ex, sm)) exsm.1 exsm.2)).
+Proof.
+  intros P Q HPQ [ex sm] HP ? ? ? ? ? ? ? ? ?.
+  edestruct HP as (?&?&?&?); eauto.
+Qed.
+
+Definition pure_wptp {Λ M} (φ : execution_trace Λ → auxiliary_trace M → Prop) :=
+  λ ex sm,
+  GFX (λ ψ (exsm : execution_trace Λ * auxiliary_trace M),
+       (pure_wptp_pre φ (λ ex sm, ψ (ex, sm)) exsm.1 exsm.2)) (ex, sm).
+
+Theorem wp_strong_adequacy Σ M Λ `{!invPreG Σ}
+        (s: stuckness) (φ : execution_trace Λ → auxiliary_trace M → Prop) e1 σ1 κs st :
+  (∀ st, smaller_card (sig (λ st', st' = st ∨ M st st')) nat) →
+  (∀ `{Hinv : !invG Σ},
+    ⊢ |={⊤}=> ∃
+         (stateI : state Λ → list (observation Λ) → nat → M → iProp Σ)
+         (Φ fork_post : val Λ → iProp Σ),
+       let _ : irisG Λ Σ M := IrisG _ _ _ Hinv stateI fork_post in
+       stateI σ1 κs 0 st ∗
+       WP e1 @ s; ⊤ {{ Φ }} ∗
+       □ (∀ (ex : execution_trace Λ) (sm : auxiliary_trace M) st' st'' c κ κs' t2 e2 t2' σ2,
+         ⌜exec_starts_in ex ([e1], σ1)⌝ -∗
+         ⌜sim_starts_in sm st⌝ -∗
+         ⌜exec_ends_in ex c⌝ -∗
+         ⌜sim_ends_in sm st'⌝ -∗
+         ⌜φ ex sm⌝ -∗
+         ⌜step c κ (t2, σ2)⌝ -∗
+         ⌜st'' = st' ∨ M st' st''⌝ -∗
+         ⌜t2 = e2 :: t2'⌝ -∗
+         ⌜∀ e2, s = NotStuck → e2 ∈ t2 → not_stuck e2 σ2⌝ -∗
+         stateI σ2 (κs' ++ κ) (length t2') st'' -∗
+         from_option Φ True (to_val e2) -∗
+         ([∗ list] v ∈ omap to_val t2', fork_post v) -∗
+         |={⊤, ∅}=>
+          ⌜ φ (exec_extend ex (t2, σ2) κ) (sim_extend sm st'') ⌝)) →
+  pure_wptp φ (singleton_exec ([e1], σ1)) (singleton_sim st).
+Proof.
+  intros Hsc Hwptp%wp_strong_adequacy_helper; last done.
+  exists (λ exsm, ⊢ wptp Σ M s φ exsm.1 exsm.2); split; first done.
+  clear Hwptp.
+  intros [ex sm] Hwptp; simpl.
+  intros Hvl Hφ c c' κ st' Hsmends Hsimends Hstep.
+  revert Hwptp.
+  rewrite {1}/wptp (fixpoint_unfold (wptp_pre _ _ _ _) _ _); intros Hwptp;
+    simpl in *.
+  apply (extract_impl ⌜_⌝) in Hwptp; last by apply extract_pure.
+  apply (extract_impl ⌜_⌝) in Hwptp; last by apply extract_pure.
+  revert Hwptp; rewrite extract_forall; intros Hwptp.
+  specialize (Hwptp c).
+  revert Hwptp; rewrite extract_forall; intros Hwptp.
+  specialize (Hwptp c').
+  revert Hwptp; rewrite extract_forall; intros Hwptp.
+  specialize (Hwptp κ).
+  revert Hwptp; rewrite extract_forall; intros Hwptp.
+  specialize (Hwptp st').
+  apply (extract_impl ⌜_⌝) in Hwptp; last by apply extract_pure.
+  apply (extract_impl ⌜_⌝) in Hwptp; last by apply extract_pure.
+  apply (extract_impl ⌜_⌝) in Hwptp; last by apply extract_pure.
+  revert Hwptp; rewrite !extract_later; intros Hwptp.
+  apply extract_exists_alt in Hwptp as [st'' Hwptp]; last done.
+  exists st''.
+  revert Hwptp.
+  rewrite !extract_and.
+  rewrite !extract_pure; done.
+Qed.
+
+
+
+
+
+
+
+
+
+
+
+
+
+
+
+
+
+
+
+
+
+
+
+
+
+
+
+
+
+
+
+
+
+
+
+
+
+
+
+
+
+
+
+
+
+
+
+
+
+
+
+
 From iris.algebra Require Import gmap auth agree gset coPset.
 From iris.proofmode Require Import tactics.
 From iris.base_logic.lib Require Import wsat.
@@ -16,87 +656,95 @@ Implicit Types Φs : list (val Λ → iProp Σ).
 Notation wptp s t Φs := ([∗ list] e;Φ ∈ t;Φs, WP e @ s; ⊤ {{ Φ }})%I.
 
 Definition config_wp : iProp Σ :=
-  (□ ∀ σ1 κ σ2 κs nt,
+  (□ ∀ σ1 δ1 κ σ2 κs nt,
         ⌜config_step σ1 κ σ2⌝ →
-        state_interp σ1 (κ ++ κs) nt ={⊤}[∅]▷=∗ state_interp σ2 κs nt).
+        state_interp σ1 δ1 κs nt ={⊤}[∅]▷=∗
+          ∃ δ2, ⌜state_variant σ1 δ1 σ2 δ2⌝ ∗ state_interp σ2 δ2 (κs ++ κ) nt).
 
-Lemma wp_step s e1 σ1 κ κs e2 σ2 efs nt Φ :
+Lemma wp_step s e1 σ1 δ1 κ κs e2 σ2 efs nt Φ :
   prim_step e1 σ1 κ e2 σ2 efs →
-  state_interp σ1 (κ ++ κs) nt -∗ WP e1 @ s; ⊤ {{ Φ }} ={⊤}[∅]▷=∗
-    state_interp σ2 κs (nt + length efs) ∗ WP e2 @ s; ⊤ {{ Φ }} ∗
+  state_interp σ1 δ1 κs nt -∗ WP e1 @ s; ⊤ {{ Φ }} ={⊤}[∅]▷=∗
+    ∃ δ2, ⌜state_variant σ1 δ1 σ2 δ2⌝ ∗
+    state_interp σ2 δ2 (κs ++ κ) (nt + length efs) ∗ WP e2 @ s; ⊤ {{ Φ }} ∗
     wptp s efs (replicate (length efs) fork_post).
 Proof.
   rewrite {1}wp_unfold /wp_pre. iIntros (?) "Hσ H".
   rewrite (val_stuck e1 σ1 κ e2 σ2 efs) //.
   iMod ("H" $! σ1 with "Hσ") as "(_ & H)".
   iMod ("H" $! e2 σ2 efs with "[//]") as "H".
-  by rewrite Nat.add_comm big_sepL2_replicate_r.
+  rewrite Nat.add_comm; setoid_rewrite big_sepL2_replicate_r; done.
 Qed.
 
-Lemma wptp_step s es1 es2 κ κs σ1 σ2 Φs nt :
+Lemma wptp_step s es1 es2 κ κs σ1 δ1 σ2 Φs nt :
   step (es1,σ1) κ (es2, σ2) →
   config_wp -∗
-  state_interp σ1 (κ ++ κs) nt -∗ wptp s es1 Φs -∗
-  ∃ nt', |={⊤}[∅]▷=> state_interp σ2 κs (nt + nt') ∗
-         wptp s es2 (Φs ++ replicate nt' fork_post).
+  state_interp σ1 δ1 κs nt -∗ wptp s es1 Φs -∗
+  ∃ nt', |={⊤}[∅]▷=>
+        ∃ δ2, ⌜state_variant σ1 δ1 σ2 δ2⌝ ∗
+          state_interp σ2 δ2 (κs ++ κ) (nt + nt') ∗
+          wptp s es2 (Φs ++ replicate nt' fork_post).
 Proof.
   iIntros (Hstep) "Hcfgwp Hσ Ht".
   destruct Hstep as [e1' σ1' e2' σ2' efs t2' t3 Hstep|]; simplify_eq/=.
   - iDestruct (big_sepL2_app_inv_l with "Ht") as (Φs1 Φs2 ->) "[? Ht]".
     iDestruct (big_sepL2_cons_inv_l with "Ht") as (Φ Φs3 ->) "[Ht ?]".
     iExists _. iMod (wp_step with "Hσ Ht") as "H"; first done.
-    iIntros "!> !>". iMod "H" as "($ & He2 & Hefs)". iIntros "!>".
+    iIntros "!> !>". iMod "H" as (δ2) "(Hsv & Hσ & He2 & Hefs)". iIntros "!>".
+    iExists δ2; iSplit; first done.
     rewrite -(assoc_L app) -app_comm_cons. iFrame.
   - iExists 0.
     iMod ("Hcfgwp" with "[] Hσ") as "Hσ"; first done.
     iModIntro; iNext; iMod "Hσ"; iModIntro.
-    rewrite right_id_L Nat.add_0_r; iFrame.
+    rewrite right_id_L Nat.add_0_r; iFrame; eauto.
 Qed.
 
-Lemma wptp_steps s n es1 es2 κs κs' σ1 σ2 Φs nt :
+Lemma wptp_steps s n es1 es2 κs κs' σ1 δ1 σ2 Φs nt :
   nsteps n (es1, σ1) κs (es2, σ2) →
-  config_wp -∗ state_interp σ1 (κs ++ κs') nt -∗ wptp s es1 Φs
-  ={⊤}[∅]▷=∗^n ∃ nt',
-    state_interp σ2 κs' (nt + nt') ∗ wptp s es2 (Φs ++ replicate nt' fork_post).
+  config_wp -∗ state_interp σ1 δ1 κs' nt -∗ wptp s es1 Φs
+  ={⊤}[∅]▷=∗^n ∃ nt' δ2,
+    state_interp σ2 δ2 (κs' ++ κs) (nt + nt') ∗ wptp s es2 (Φs ++ replicate nt' fork_post).
 Proof.
-  revert nt es1 es2 κs κs' σ1 σ2 Φs.
-  induction n as [|n IH]=> nt es1 es2 κs κs' σ1 σ2 Φs /=.
-  { inversion_clear 1; iIntros "? ? ?"; iExists 0=> /=.
-    rewrite Nat.add_0_r right_id_L. by iFrame. }
+  revert nt es1 es2 κs κs' σ1 δ1 σ2 Φs.
+  induction n as [|n IH]=> nt es1 es2 κs κs' σ1 δ1 σ2 Φs /=.
+  { inversion_clear 1; iIntros "? ? ?"; iExists 0, δ1 => /=.
+    rewrite Nat.add_0_r !right_id_L. by iFrame. }
   iIntros (Hsteps) "#Hcfgwp Hσ He". inversion_clear Hsteps as [|?? [t1' σ1']].
-  rewrite -(assoc_L (++)).
   iDestruct (wptp_step with "[] Hσ He") as (nt') ">H"; [done|done|]; simplify_eq.
-  iIntros "!> !>". iMod "H" as "(Hσ & He)". iModIntro.
-  iApply (step_fupdN_wand with "[Hσ He]"); first by iApply (IH with "[] Hσ He").
-  iDestruct 1 as (nt'') "[??]".
+  iIntros "!> !>". iMod "H" as (δ2) "(Hsv & Hσ & He)". iModIntro.
+  iApply (step_fupdN_wand with "[Hσ He]").
+  { by iApply (IH with "[] Hσ He"). }
+  iDestruct 1 as (nt'' δ3) "[??]".
+  rewrite -(assoc_L (++)).
   rewrite -Nat.add_assoc -(assoc_L app) -replicate_plus.
   by eauto with iFrame.
 Qed.
 
-Lemma wp_not_stuck κs nt e σ Φ :
-  state_interp σ κs nt -∗ WP e {{ Φ }} ={⊤}=∗ ⌜not_stuck e σ⌝.
+Lemma wp_not_stuck κs nt e σ δ Φ :
+  state_interp σ δ κs nt -∗ WP e {{ Φ }} ={⊤}=∗ ⌜not_stuck e σ⌝.
 Proof.
   rewrite wp_unfold /wp_pre /not_stuck. iIntros "Hσ H".
   destruct (to_val e) as [v|] eqn:?; first by eauto.
-  iSpecialize ("H" $! σ [] κs with "Hσ"). rewrite sep_elim_l.
+  iSpecialize ("H" $! σ δ [] κs with "Hσ"). rewrite sep_elim_l.
   iMod (fupd_plain_mask with "H") as %?; eauto.
 Qed.
 
-Lemma wptp_strong_adequacy Φs κs' s n es1 es2 κs σ1 σ2 nt:
+Lemma wptp_strong_adequacy Φs κs' s n es1 es2 κs σ1 δ1 σ2 nt:
   nsteps n (es1, σ1) κs (es2, σ2) →
-  config_wp -∗ state_interp σ1 (κs ++ κs') nt -∗
-  wptp s es1 Φs ={⊤}[∅]▷=∗^(S n) ∃ nt',
+  config_wp -∗ state_interp σ1 δ1 κs' nt -∗
+  wptp s es1 Φs ={⊤}[∅]▷=∗^(S n) ∃ nt' δ2,
     ⌜ ∀ e2, s = NotStuck → e2 ∈ es2 → not_stuck e2 σ2 ⌝ ∗
-    state_interp σ2 κs' (nt + nt') ∗
-    [∗ list] e;Φ ∈ es2;Φs ++ replicate nt' fork_post, from_option Φ True (to_val e).
+    state_interp σ2 δ2 (κs' ++ κs) (nt + nt') ∗
+    [∗ list] e;Φ ∈ es2;Φs ++ replicate nt' fork_post,
+      from_option Φ True (to_val e).
 Proof.
   iIntros (Hstep) "#Hcfgwp Hσ He". rewrite Nat_iter_S_r.
   iDestruct (wptp_steps with "[] Hσ He") as "Hwp"; [done|done|].
   iApply (step_fupdN_wand with "Hwp").
-  iDestruct 1 as (nt') "(Hσ & Ht)"; simplify_eq/=.
+  iDestruct 1 as (nt' δ2) "(Hσ & Ht)"; simplify_eq/=.
   iMod (fupd_plain_keep_l ⊤
     ⌜ ∀ e2, s = NotStuck → e2 ∈ es2 → not_stuck e2 σ2 ⌝%I
-    (state_interp σ2 κs' (nt + nt') ∗ wptp s es2 (Φs ++ replicate nt' fork_post))%I
+    (state_interp σ2 δ2 (κs' ++ κs) (nt + nt') ∗
+    wptp s es2 (Φs ++ replicate nt' fork_post))%I
     with "[$Hσ $Ht]") as "(%&Hσ&Hwp)".
   { iIntros "(Hσ & Ht)" (e' -> He').
     move: He' => /(elem_of_list_split _ _)[?[?->]].
@@ -104,7 +752,7 @@ Proof.
     iDestruct (big_sepL2_cons_inv_l with "Hwp") as (Φ Φs3 ->) "[Hwp ?]".
     iMod (wp_not_stuck with "Hσ Hwp") as "$"; auto. }
   iApply step_fupd_fupd. iApply step_fupd_intro; first done. iNext.
-  iExists _. iSplitR; first done. iFrame "Hσ".
+  iExists _, _. iSplitR; first done. iFrame "Hσ".
   iApply big_sepL2_fupd.
   iApply (big_sepL2_impl with "Hwp").
   iIntros "!#" (? e Φ ??) "Hwp".
